####Part a:
Using Gaussian quadrature, we let:
$$\int_a^b f(x) dx=c_0f(x_0)+c_1f(x_1)+c_2f(x_2)$$
Now, let $a=x_i$, $b=x_i + h$, $x_0 = \frac{h}{3}$, $x_1 = \frac{h}{2}$, $x_2 = \frac{2h}{3}$  

Using basis functions: 
$$f(x)=1$$
$$f(x)=x$$
$$f(x)=x^2$$
Considering $f(x) = x^n$ for $n > 0$:
$$let \space I_n = \int_{x_i}^{x_i + h}f(x)dx$$
$$= \int_{x_i}^{x_i + h}x^ndx$$
$$=\frac{1}{n+1}[(x_i+h)^{n+1}-x_i^{n+1}]$$
$$=c_0(x_i+\frac{h}{3})^n + c_1(x_i+\frac{h}{2})^n + c_2(x_i+\frac{2h}{3})^n$$
Then:
$$I_0 = h = c_0 + c_1 + c_2$$
$$I_1 =\frac{1}{2}[(x_i+h)^{2}-x_i^2] = c_0(x_i+\frac{h}{3}) + c_1(x_i+\frac{h}{2}) + c_2(x_i+\frac{2h}{3})$$
$$I_2 =\frac{1}{3}[(x_i+h)^{3}-x_i^3]= c_0(x_i+\frac{h}{3})^2 + c_1(x_i+\frac{h}{2})^2 + c_2(x_i+\frac{2h}{3})^2$$
This gives the following linear system:
$$
\left[ \mkern1mu \begin{array}{@{}ccc|c@{}}
1 & 1 & 1 & h \\
(x_i+\frac{h}{3}) & (x_i+\frac{h}{2}) & (x_i+\frac{2h}{3}) & \frac{1}{2}[(x_i+h)^{2}-x_i^2] \\
(x_i+\frac{h}{3})^2 & (x_i+\frac{h}{2})^2 & (x_i+\frac{2h}{3})^2 & \frac{1}{3}[(x_i+h)^{3}-x_i^3]
\end{array} \mkern1mu \right]
$$
Applying 
- $R2\rightarrow R2 - (x_i+\frac{h}{3})R1$
- $R3\rightarrow R3 - (x_i+\frac{h}{3})^2R1$
We get:
$$
\left[ \mkern1mu \begin{array}{@{}ccc|c@{}}
1 & 1 & 1 & h \\
0 & (x_i+\frac{h}{2}) - (x_i+\frac{h}{3}) & (x_i+\frac{2h}{3}) - (x_i+\frac{h}{3}) & \frac{1}{2}[(x_i+h)^{2}-x_i^2] - h(x_i+\frac{h}{3}) \\
0 & (x_i+\frac{h}{2})^2-(x_i+\frac{h}{3})^2 & (x_i+\frac{2h}{3})^2 - (x_i+\frac{h}{3})^2& \frac{1}{3}[(x_i+h)^{3}-x_i^3] - h(x_i+\frac{h}{3})^2
\end{array} \mkern1mu \right]
$$
$$
=\left[ \mkern1mu \begin{array}{@{}ccc|c@{}}
1 & 1 & 1 & h \\
0 & \frac{h}{6} & \frac{h}{3} & \frac{h^2}{6} \\
0 & \frac{1}{3}x_ih + \frac{5}{36}h^2 & \frac{2}{3}x_ih + \frac{1}{3}h^2 & \frac{1}{3}x_ih^2 + \frac{4}{9}h^3
\end{array} \mkern1mu \right]
$$
Applying 
- $R2 \rightarrow \frac{6}{h}R2$ 
- $R3 \rightarrow \frac{9}{h}R2$
Yields:
$$
\left[ \mkern1mu \begin{array}{@{}ccc|c@{}}
1 & 1 & 1 & h \\
0 & 1 & 2 & h \\
0 & 3x_i + \frac{5}{4}h & 6x_i + 3h & 3x_ih + 4h^2
\end{array} \mkern1mu \right]
$$
Applying $R3\rightarrow R3 - (3x_i + \frac{5}{4}h)R2$ yields:
$$
\left[ \mkern1mu \begin{array}{@{}ccc|c@{}}
1 & 1 & 1 & h \\
0 & 1 & 2 & h \\
0 & 0 & 6x_i + 3h - 2 (3x_i + \frac{5}{4}h) & 3x_ih + 4h^2 - h(3x_i + \frac{5}{4}h)
\end{array} \mkern1mu \right]
$$
$$
=\left[ \mkern1mu \begin{array}{@{}ccc|c@{}}
1 & 1 & 1 & h \\
0 & 1 & 2 & h \\
0 & 0 & \frac{1}{2}h &\frac{11}{4}h^2
\end{array} \mkern1mu \right]
$$
Thus:
$$
\frac{1}{2}hc_3 = \frac{11}{4}h^2
\implies c_3 = \frac{11}{2}h
$$
$$c_1 + 2c_2 = h \implies c_1 = h - 2(\frac{11}{2}h) = -10h$$
$$c_0 + c_1 + c_2 = h \implies c_0 = h - (-10h) -(\frac{11}{2}h) = \frac{11}{2}h$$
Therefore:
$$\int_{x_i}^{x_i + h}f(x)dx\approx \frac{11}{2}h(x_i+\frac{h}{3}) + -10hc_1(x_i+\frac{h}{2}) +\frac{11}{2}hc_2(x_i+\frac{2h}{3})$$
####Part b:
It is known that a quadrature rule with n + 1 nodes cannot be exact for all polynomials of 
degree ≤ 2n + 2. 

However, Gaussian quadrature is exact for all polynomials of degree ≤ 2n - 1.

For the rule above, there are 3 nodes so n = 2. Thus as it is derived using Gaussian quadrature, it is correct for all polynomials of degree ≤ 5.

####Part c:
